{
  "@context": {
    "problem": "https://tools.ietf.org/html/rfcXXXX/vocab#",
    "rdf": "http://www.w3.org/1999/02/22-rdf-syntax-ns#",
    "rdfs": "http://www.w3.org/2000/01/rdf-schema#",
    "xsd": "http://www.w3.org/2001/XMLSchema#",
    "owl": "http://www.w3.org/2002/07/owl#",
    "defines": {
      "@reverse": "rdfs:isDefinedBy"
    },
    "rdfs:domain": {
      "@type": "@id"
    },
    "rdfs:range": {
      "@type": "@id"
    },
    "rdfs:subClassOf": {
      "@type": "@id"
    }
  },
  "@id": "https://tools.ietf.org/html/rfcXXXX/vocab",
  "@type": "owl:Ontology",
  "comment": "This document defines a 'problem detail' vocabulary as a way to carry machine-readable details of errors in a HTTP response, to avoid the need to invent new error response formats for HTTP APIs.",
  "rdfs:label": "Problem Details for HTTP APIs",
  "defines": [
    {
      "@id": "problem:HttpProblem",
      "@type": "rdfs:Class",
      "rdfs:comment": "The class of http problem detail descriptions",
      "rdfs:subClassOf": [
        "rdfs:Resource"
      ]
    },
    {
      "@id": "problem:instance",
      "@type": "xsd:string",
      "rdfs:comment": "A URI reference that identifies the specific occurrence of the problem",
      "rdfs:domain": "problem:HttpProblem",
      "rdfs:range": "xsd:string"
    },
    {
      "@id": "problem:title",
      "@type": "rdf:Property",
      "rdfs:comment": "A short, human-readable summary of the problem type",
      "rdfs:domain": "problem:HttpProblem",
      "rdfs:range": "xsd:string"
    },
    {
      "@id": "problem:status",
      "@type": "rdf:Property",
      "rdfs:comment": "The HTTP status code ([RFC7231], Section 6)",
      "rdfs:domain": "problem:HttpProblem",
      "rdfs:range": "xsd:integer"
    },
    {
      "@id": "problem:detail",
      "@type": "rdf:Property",
      "rdfs:comment": "A human readable explanation specific to this occurence of the problem",
      "rdfs:domain": "problem:HttpProblem",
      "rdfs:range": "xsd:string"
    },
    {
      "@id": "problem:type",
      "@type": "xsd:string",
      "rdfs:comment": "A URI reference [RFC3986] that identifies the problem type. When this member is not present, its value is assumed to be 'about:blank'",
      "rdfs:domain": "problem:HttpProblem",
      "rdfs:range": "xsd:string"
    }
  ]
}